playground/uart_model/NOTE_HANDL_CODE_WORD.sml
@@ -1,0 +1,69 @@
+open m0u_progTheory;
+open Int;
+open m0_decompLib;
+open m0Theory;
+open progSyntax;
+open pairLib;
+open pred_setSyntax;
+open m0_progLib;
+open m0_stepLib;
+open wordsSyntax;
+open progTheory;
+open m0_progTheory;
+
+ 
+val (code_th, code_defs) = m0_decompile "code"` 
+  00c0
+  1814
+  5ce5
+`;
+(* to extend code pool with .word 0xabcdfff after the last instruction*)
+(* by extending the code pool with  (p+6w, data_to_thumb2 (0xabcdefffw)) *)
+
+(* Need the fact that extending code with .WORD is a subset  *)
+val CODE_SUB = prove(``{(p,INL 192w); (p + 2w,INL 6164w); (p + 4w,INL 23781w)} SUBSET {(p,INL 192w); (p + 2w,INL 6164w); (p + 4w,INL 23781w); (p+6w, data_to_thumb2 (0xabcdefffw))}``,
+    SIMP_TAC (std_ss++pred_setLib.PRED_SET_ss) [] );
+
+
+(* Need the fact that .word is disjoint from the rest of the code *)
+
+val CODE_DISJOINT_TAC = 
+(REV_FULL_SIMP_TAC (std_ss++pred_setLib.PRED_SET_ss) [PULL_EXISTS, m0_instr_def, data_to_thumb2_def]>>
+REPEAT STRIP_TAC>>(
+    REV_FULL_SIMP_TAC (std_ss++pred_setLib.PRED_SET_ss) [PULL_EXISTS, m0_instr_def, data_to_thumb2_def]>>
+    EVAL_TAC))
+
+
+val CODE_DISJOINT = prove(`` (DISJOINT (m0_instr (p+6w, data_to_thumb2 (0xabcdefffw)))
+                 (BIGUNION (IMAGE m0_instr {(p,INL 192w); (p + 2w,INL 6164w); (p + 4w,INL 23781w)} )))``, CODE_DISJOINT_TAC)
+
+(* Now we should be able to extend the code using 
+
+    (("prog", "SPEC_SUBSET_CODE"),
+     ( [] ⊢ ∀x p c q. SPEC x p c q ⇒ ∀c'. c ⊆ c' ⇒ SPEC x p c' q, Thm)),
+
+   AND we cane move data back and froth from conditions to code using:
+
+    (("m0_prog", "MOVE_TO_M0_CODE_POOL"),
+	( []
+	⊢ ∀a w c p q.
+		SPEC M0_MODEL
+		(p * m0_MEM a ((7 >< 0) w) * m0_MEM (a + 1w) ((15 >< 8) w) *
+		m0_MEM (a + 2w) ((23 >< 16) w) *
+		m0_MEM (a + 3w) ((31 >< 24) w)) c
+		(q * m0_MEM a ((7 >< 0) w) * m0_MEM (a + 1w) ((15 >< 8) w) *
+		m0_MEM (a + 2w) ((23 >< 16) w) *
+		m0_MEM (a + 3w) ((31 >< 24) w)) ⇔
+		SPEC M0_MODEL
+		(cond
+		    (DISJOINT (m0_instr (a,data_to_thumb2 w))
+			(BIGUNION (IMAGE m0_instr c))) * p)
+		((a,data_to_thumb2 w) INSERT c) q, Thm)),
+
+
+   But i suspect that the worklfow will be something like: 
+   1) decompile 
+   2) factor out the data in pre and post conditions
+   3) use above stuff to move data into code
+   4) check that data matches .word in content and address 
+*)
