playground/uart_model/VC_experement.sml
@@ -1,0 +1,43 @@
+open m0u_progTheory;
+open Int;
+open m0_decompLib;
+open m0Theory;
+open progSyntax;
+open pairLib;
+open pred_setSyntax;
+open m0_progLib;
+open m0_stepLib;
+open wordsSyntax;
+ 
+thumb_decode_hex false "0000  "
+ 
+register_instruction
+ 
+val (code_th, code_defs) = m0_decompile "code"` 
+  00c0
+  1814
+  5ce5
+`;
+
+val   code2_thm =  m0_spec_hex "f7ffffb9"
+m0_spec_hex "00C0"
+``0xffffw``
+
+ open m0_progLib;
+	  m0_get_code ``(p,INL 192w)``
+
+get_code (m0_spec "BL")
+
+m0_sp
+
+(( fmt StringCvt.HEX o uint_of_word o snd o  dest_comb o  snd o  dest_pair o  hd o strip_set o  #3 o  dest_spec o concl) code_th) 
+    
+case (( dest_comb o  snd o  dest_pair o  hd o strip_set o  #3 o  dest_spec o concl) code_th) of
+    ("INL", inst) => uint_of_word inst 
+  | ("INR", inst) => uint_of_word inst;
+
+
+
+dest_prod
+
+dist_pair inst
