playground/uart_model/m0u_progTheory.sig
@@ -1,0 +1,414 @@
+signature m0u_progTheory =
+sig
+  type thm = Thm.thm
+  
+  (*  Definitions  *)
+    val COSIM_def : thm
+    val M0U_MODEL_def : thm
+    val NextStateM0U_def : thm
+    val SDOM_def : thm
+    val TO_M0U_PROP_def : thm
+    val TO_M0U_def : thm
+    val m0u_component_TY_DEF : thm
+    val m0u_component_case_def : thm
+    val m0u_component_size_def : thm
+    val m0u_data_TY_DEF : thm
+    val m0u_data_case_def : thm
+    val m0u_data_size_def : thm
+    val m0u_proj_def : thm
+    val r2m0_c_set_def : thm
+  
+  (*  Theorems  *)
+    val NEX_thm : thm
+    val NIT_COSIM_thm : thm
+    val NIT_NIT_STEP_thm : thm
+    val TP_def : thm
+    val WS_COSIM_thm : thm
+    val datatype_m0u_component : thm
+    val datatype_m0u_data : thm
+    val m0u_component_11 : thm
+    val m0u_component_Axiom : thm
+    val m0u_component_case_cong : thm
+    val m0u_component_case_eq : thm
+    val m0u_component_distinct : thm
+    val m0u_component_induction : thm
+    val m0u_component_nchotomy : thm
+    val m0u_data_11 : thm
+    val m0u_data_Axiom : thm
+    val m0u_data_case_cong : thm
+    val m0u_data_case_eq : thm
+    val m0u_data_distinct : thm
+    val m0u_data_induction : thm
+    val m0u_data_nchotomy : thm
+  
+  val m0u_prog_grammars : type_grammar.grammar * term_grammar.grammar
+(*
+   [clock] Parent theory of "m0u_prog"
+   
+   [uart] Parent theory of "m0u_prog"
+   
+   [COSIM_def]  Definition
+      
+       []
+      ⊢ ∀P t.
+            COSIM P t ⇔
+            ∀s s' seq seq' i.
+                SEP_REFINE (P * SEP_T) $= (STATE m0_proj) s ∧
+                rel_sequence (NEXT_REL $= NextStateM0) seq s ∧
+                rel_sequence (NEXT_REL $= NextStateM0U) seq' s' ∧
+                ¬((SND ∘ FST) s').unpredictable ∧
+                m0u_m0_non_r_eq uart_r s' s ∧ (seq i).count ≤ s.count + t ⇒
+                m0u_m0_non_r_eq uart_r (seq' i) (seq i) ∧
+                m0u_r_eq uart_r s' (seq' i)
+   
+   [M0U_MODEL_def]  Definition
+      
+       []
+      ⊢ M0U_MODEL =
+        (STATE m0u_proj,NEXT_REL $= NextStateM0U,(λc. TO_M0U (m0_instr c)),
+         $=,K F)
+   
+   [NextStateM0U_def]  Definition
+      
+       []
+      ⊢ ∀s0.
+            NextStateM0U s0 =
+            (let
+               s1 = m0u_Next s0
+             in
+               if
+                 ¬((SND ∘ FST) s1).unpredictable ∧
+                 (((FST ∘ FST) s1).exception = NoException)
+               then
+                 SOME s1 else NONE)
+   
+   [SDOM_def]  Definition
+      
+       [] ⊢ ∀A. SDOM A = BIGUNION (IMAGE (IMAGE (λ(c,_). c)) A)
+   
+   [TO_M0U_PROP_def]  Definition
+      
+       [] ⊢ TO_M0U_PROP = IMAGE TO_M0U
+   
+   [TO_M0U_def]  Definition
+      
+       [] ⊢ TO_M0U = IMAGE (m0_c ## m0_d)
+   
+   [m0u_component_TY_DEF]  Definition
+      
+       []
+      ⊢ ∃rep.
+            TYPE_DEFINITION
+              (λa0.
+                   ∀'m0u_component' .
+                       (∀a0.
+                            (∃a.
+                                 a0 =
+                                 (λa.
+                                      ind_type$CONSTR 0 a
+                                        (λn. ind_type$BOTTOM)) a) ∨
+                            (a0 =
+                             ind_type$CONSTR (SUC 0) ARB
+                               (λn. ind_type$BOTTOM)) ∨
+                            (a0 =
+                             ind_type$CONSTR (SUC (SUC 0)) ARB
+                               (λn. ind_type$BOTTOM)) ∨
+                            (a0 =
+                             ind_type$CONSTR (SUC (SUC (SUC 0))) ARB
+                               (λn. ind_type$BOTTOM)) ∨
+                            (a0 =
+                             ind_type$CONSTR (SUC (SUC (SUC (SUC 0)))) ARB
+                               (λn. ind_type$BOTTOM)) ∨
+                            (a0 =
+                             ind_type$CONSTR
+                               (SUC (SUC (SUC (SUC (SUC 0))))) ARB
+                               (λn. ind_type$BOTTOM)) ∨
+                            (a0 =
+                             ind_type$CONSTR
+                               (SUC (SUC (SUC (SUC (SUC (SUC 0)))))) ARB
+                               (λn. ind_type$BOTTOM)) ⇒
+                            'm0u_component' a0) ⇒
+                       'm0u_component' a0) rep
+   
+   [m0u_component_case_def]  Definition
+      
+       []
+      ⊢ (∀a f v v1 v2 v3 v4 v5.
+             m0u_component_CASE (m0_c a) f v v1 v2 v3 v4 v5 = f a) ∧
+        (∀f v v1 v2 v3 v4 v5.
+             m0u_component_CASE m0u_c_Input f v v1 v2 v3 v4 v5 = v) ∧
+        (∀f v v1 v2 v3 v4 v5.
+             m0u_component_CASE m0u_c_Output f v v1 v2 v3 v4 v5 = v1) ∧
+        (∀f v v1 v2 v3 v4 v5.
+             m0u_component_CASE m0u_c_RXD f v v1 v2 v3 v4 v5 = v2) ∧
+        (∀f v v1 v2 v3 v4 v5.
+             m0u_component_CASE m0u_c_TXD f v v1 v2 v3 v4 v5 = v3) ∧
+        (∀f v v1 v2 v3 v4 v5.
+             m0u_component_CASE m0u_c_RXDRDY f v v1 v2 v3 v4 v5 = v4) ∧
+        ∀f v v1 v2 v3 v4 v5.
+            m0u_component_CASE m0u_c_TXDRDY f v v1 v2 v3 v4 v5 = v5
+   
+   [m0u_component_size_def]  Definition
+      
+       []
+      ⊢ (∀a. m0u_component_size (m0_c a) = 1 + m0_component_size a) ∧
+        (m0u_component_size m0u_c_Input = 0) ∧
+        (m0u_component_size m0u_c_Output = 0) ∧
+        (m0u_component_size m0u_c_RXD = 0) ∧
+        (m0u_component_size m0u_c_TXD = 0) ∧
+        (m0u_component_size m0u_c_RXDRDY = 0) ∧
+        (m0u_component_size m0u_c_TXDRDY = 0)
+   
+   [m0u_data_TY_DEF]  Definition
+      
+       []
+      ⊢ ∃rep.
+            TYPE_DEFINITION
+              (λa0.
+                   ∀'m0u_data' .
+                       (∀a0.
+                            (∃a.
+                                 a0 =
+                                 (λa.
+                                      ind_type$CONSTR 0 (a,ARB,ARB,ARB)
+                                        (λn. ind_type$BOTTOM)) a) ∨
+                            (∃a.
+                                 a0 =
+                                 (λa.
+                                      ind_type$CONSTR (SUC 0)
+                                        (ARB,a,ARB,ARB)
+                                        (λn. ind_type$BOTTOM)) a) ∨
+                            (∃a.
+                                 a0 =
+                                 (λa.
+                                      ind_type$CONSTR (SUC (SUC 0))
+                                        (ARB,ARB,a,ARB)
+                                        (λn. ind_type$BOTTOM)) a) ∨
+                            (∃a.
+                                 a0 =
+                                 (λa.
+                                      ind_type$CONSTR (SUC (SUC (SUC 0)))
+                                        (ARB,ARB,ARB,a)
+                                        (λn. ind_type$BOTTOM)) a) ⇒
+                            'm0u_data' a0) ⇒
+                       'm0u_data' a0) rep
+   
+   [m0u_data_case_def]  Definition
+      
+       []
+      ⊢ (∀a f f1 f2 f3. m0u_data_CASE (m0_d a) f f1 f2 f3 = f a) ∧
+        (∀a f f1 f2 f3. m0u_data_CASE (m0u_d_stream a) f f1 f2 f3 = f1 a) ∧
+        (∀a f f1 f2 f3. m0u_data_CASE (m0u_d_word32 a) f f1 f2 f3 = f2 a) ∧
+        ∀a f f1 f2 f3. m0u_data_CASE (m0u_d_bool a) f f1 f2 f3 = f3 a
+   
+   [m0u_data_size_def]  Definition
+      
+       []
+      ⊢ (∀a. m0u_data_size (m0_d a) = 1 + m0_data_size a) ∧
+        (∀a. m0u_data_size (m0u_d_stream a) = 1 + list_size (λv. 0) a) ∧
+        (∀a. m0u_data_size (m0u_d_word32 a) = 1) ∧
+        ∀a. m0u_data_size (m0u_d_bool a) = 1 + bool_size a
+   
+   [m0u_proj_def]  Definition
+      
+       []
+      ⊢ ∀s u input output.
+            m0u_proj ((s,u),input,output) =
+            (λa.
+                 case a of
+                   m0_c b => m0_d (m0_proj s b)
+                 | m0u_c_Input => m0u_d_stream input
+                 | m0u_c_Output => m0u_d_stream output
+                 | m0u_c_RXD => m0u_d_word32 u.RXD
+                 | m0u_c_TXD => m0u_d_word32 u.RXD
+                 | m0u_c_RXDRDY => m0u_d_word32 u.RXD
+                 | m0u_c_TXDRDY => m0u_d_word32 u.RXD)
+   
+   [r2m0_c_set_def]  Definition
+      
+       [] ⊢ ∀region. r2m0_c_set region = IMAGE m0_c_MEM region
+   
+   [NEX_thm]  Theorem
+      
+       []
+      ⊢ ∀P t s seq i.
+            NEX P t ⇒
+            SEP_REFINE (P * SEP_T) $= (STATE m0_proj) s ∧
+            rel_sequence (NEXT_REL $= NextStateM0) seq s ∧
+            (seq (SUC i)).count ≤ s.count + t ⇒
+            (seq i).count < (Next (seq i)).count ∧
+            (Next (seq i) = seq (SUC i))
+   
+   [NIT_COSIM_thm]  Theorem
+      
+       [] ⊢ ∀P t. NIT uart_r P t ∧ NEX P t ⇒ COSIM P t
+   
+   [NIT_NIT_STEP_thm]  Theorem
+      
+       []
+      ⊢ ∀P t s seq i.
+            NIT uart_r P t ∧ NEX P t ⇒
+            SEP_REFINE (P * SEP_T) $= (STATE m0_proj) s ∧
+            rel_sequence (NEXT_REL $= NextStateM0) seq s ∧
+            (seq (SUC i)).count ≤ s.count + t ⇒
+            NIT_STEP uart_r (seq i)
+   
+   [TP_def]  Theorem
+      
+      [oracles: cheat] [axioms: ] []
+      ⊢ ∀P C Q c t.
+            SPEC M0_MODEL (P * m0_count c) C (Q * m0_count (c + t)) ∧
+            COSIM P t ∧ (∀SET. P SET ⇒ DISJOINT SET UART) ∧
+            (∀SET. Q SET ⇒ DISJOINT SET UART) ⇒
+            SPEC M0U_MODEL (TO_M0U_PROP (P * m0_count c)) C
+              (TO_M0U_PROP (Q * m0_count (c + t)))
+   
+   [WS_COSIM_thm]  Theorem
+      
+      [oracles: tactic_failed] [axioms: ] []
+      ⊢ ∀P P' t t'. COSIM P t ∧ t' < t ∧ SEP_IMP P' P ⇒ COSIM P' t'
+   
+   [datatype_m0u_component]  Theorem
+      
+       []
+      ⊢ DATATYPE
+          (m0u_component m0_c m0u_c_Input m0u_c_Output m0u_c_RXD m0u_c_TXD
+             m0u_c_RXDRDY m0u_c_TXDRDY)
+   
+   [datatype_m0u_data]  Theorem
+      
+       [] ⊢ DATATYPE (m0u_data m0_d m0u_d_stream m0u_d_word32 m0u_d_bool)
+   
+   [m0u_component_11]  Theorem
+      
+       [] ⊢ ∀a a'. (m0_c a = m0_c a') ⇔ (a = a')
+   
+   [m0u_component_Axiom]  Theorem
+      
+       []
+      ⊢ ∀f0 f1 f2 f3 f4 f5 f6.
+            ∃fn.
+                (∀a. fn (m0_c a) = f0 a) ∧ (fn m0u_c_Input = f1) ∧
+                (fn m0u_c_Output = f2) ∧ (fn m0u_c_RXD = f3) ∧
+                (fn m0u_c_TXD = f4) ∧ (fn m0u_c_RXDRDY = f5) ∧
+                (fn m0u_c_TXDRDY = f6)
+   
+   [m0u_component_case_cong]  Theorem
+      
+       []
+      ⊢ ∀M M' f v v1 v2 v3 v4 v5.
+            (M = M') ∧ (∀a. (M' = m0_c a) ⇒ (f a = f' a)) ∧
+            ((M' = m0u_c_Input) ⇒ (v = v')) ∧
+            ((M' = m0u_c_Output) ⇒ (v1 = v1')) ∧
+            ((M' = m0u_c_RXD) ⇒ (v2 = v2')) ∧
+            ((M' = m0u_c_TXD) ⇒ (v3 = v3')) ∧
+            ((M' = m0u_c_RXDRDY) ⇒ (v4 = v4')) ∧
+            ((M' = m0u_c_TXDRDY) ⇒ (v5 = v5')) ⇒
+            (m0u_component_CASE M f v v1 v2 v3 v4 v5 =
+             m0u_component_CASE M' f' v' v1' v2' v3' v4' v5')
+   
+   [m0u_component_case_eq]  Theorem
+      
+       []
+      ⊢ (m0u_component_CASE x f v v1 v2 v3 v4 v5 = v') ⇔
+        (∃m. (x = m0_c m) ∧ (f m = v')) ∨ (x = m0u_c_Input) ∧ (v = v') ∨
+        (x = m0u_c_Output) ∧ (v1 = v') ∨ (x = m0u_c_RXD) ∧ (v2 = v') ∨
+        (x = m0u_c_TXD) ∧ (v3 = v') ∨ (x = m0u_c_RXDRDY) ∧ (v4 = v') ∨
+        (x = m0u_c_TXDRDY) ∧ (v5 = v')
+   
+   [m0u_component_distinct]  Theorem
+      
+       []
+      ⊢ (∀a. m0_c a ≠ m0u_c_Input) ∧ (∀a. m0_c a ≠ m0u_c_Output) ∧
+        (∀a. m0_c a ≠ m0u_c_RXD) ∧ (∀a. m0_c a ≠ m0u_c_TXD) ∧
+        (∀a. m0_c a ≠ m0u_c_RXDRDY) ∧ (∀a. m0_c a ≠ m0u_c_TXDRDY) ∧
+        m0u_c_Input ≠ m0u_c_Output ∧ m0u_c_Input ≠ m0u_c_RXD ∧
+        m0u_c_Input ≠ m0u_c_TXD ∧ m0u_c_Input ≠ m0u_c_RXDRDY ∧
+        m0u_c_Input ≠ m0u_c_TXDRDY ∧ m0u_c_Output ≠ m0u_c_RXD ∧
+        m0u_c_Output ≠ m0u_c_TXD ∧ m0u_c_Output ≠ m0u_c_RXDRDY ∧
+        m0u_c_Output ≠ m0u_c_TXDRDY ∧ m0u_c_RXD ≠ m0u_c_TXD ∧
+        m0u_c_RXD ≠ m0u_c_RXDRDY ∧ m0u_c_RXD ≠ m0u_c_TXDRDY ∧
+        m0u_c_TXD ≠ m0u_c_RXDRDY ∧ m0u_c_TXD ≠ m0u_c_TXDRDY ∧
+        m0u_c_RXDRDY ≠ m0u_c_TXDRDY
+   
+   [m0u_component_induction]  Theorem
+      
+       []
+      ⊢ ∀P.
+            (∀m. P (m0_c m)) ∧ P m0u_c_Input ∧ P m0u_c_Output ∧
+            P m0u_c_RXD ∧ P m0u_c_TXD ∧ P m0u_c_RXDRDY ∧ P m0u_c_TXDRDY ⇒
+            ∀m. P m
+   
+   [m0u_component_nchotomy]  Theorem
+      
+       []
+      ⊢ ∀mm.
+            (∃m. mm = m0_c m) ∨ (mm = m0u_c_Input) ∨ (mm = m0u_c_Output) ∨
+            (mm = m0u_c_RXD) ∨ (mm = m0u_c_TXD) ∨ (mm = m0u_c_RXDRDY) ∨
+            (mm = m0u_c_TXDRDY)
+   
+   [m0u_data_11]  Theorem
+      
+       []
+      ⊢ (∀a a'. (m0_d a = m0_d a') ⇔ (a = a')) ∧
+        (∀a a'. (m0u_d_stream a = m0u_d_stream a') ⇔ (a = a')) ∧
+        (∀a a'. (m0u_d_word32 a = m0u_d_word32 a') ⇔ (a = a')) ∧
+        ∀a a'. (m0u_d_bool a = m0u_d_bool a') ⇔ (a ⇔ a')
+   
+   [m0u_data_Axiom]  Theorem
+      
+       []
+      ⊢ ∀f0 f1 f2 f3.
+            ∃fn.
+                (∀a. fn (m0_d a) = f0 a) ∧
+                (∀a. fn (m0u_d_stream a) = f1 a) ∧
+                (∀a. fn (m0u_d_word32 a) = f2 a) ∧
+                ∀a. fn (m0u_d_bool a) = f3 a
+   
+   [m0u_data_case_cong]  Theorem
+      
+       []
+      ⊢ ∀M M' f f1 f2 f3.
+            (M = M') ∧ (∀a. (M' = m0_d a) ⇒ (f a = f' a)) ∧
+            (∀a. (M' = m0u_d_stream a) ⇒ (f1 a = f1' a)) ∧
+            (∀a. (M' = m0u_d_word32 a) ⇒ (f2 a = f2' a)) ∧
+            (∀a. (M' = m0u_d_bool a) ⇒ (f3 a = f3' a)) ⇒
+            (m0u_data_CASE M f f1 f2 f3 = m0u_data_CASE M' f' f1' f2' f3')
+   
+   [m0u_data_case_eq]  Theorem
+      
+       []
+      ⊢ (m0u_data_CASE x f f1 f2 f3 = v) ⇔
+        (∃m. (x = m0_d m) ∧ (f m = v)) ∨
+        (∃l. (x = m0u_d_stream l) ∧ (f1 l = v)) ∨
+        (∃c. (x = m0u_d_word32 c) ∧ (f2 c = v)) ∨
+        ∃b. (x = m0u_d_bool b) ∧ (f3 b = v)
+   
+   [m0u_data_distinct]  Theorem
+      
+       []
+      ⊢ (∀a' a. m0_d a ≠ m0u_d_stream a') ∧
+        (∀a' a. m0_d a ≠ m0u_d_word32 a') ∧
+        (∀a' a. m0_d a ≠ m0u_d_bool a') ∧
+        (∀a' a. m0u_d_stream a ≠ m0u_d_word32 a') ∧
+        (∀a' a. m0u_d_stream a ≠ m0u_d_bool a') ∧
+        ∀a' a. m0u_d_word32 a ≠ m0u_d_bool a'
+   
+   [m0u_data_induction]  Theorem
+      
+       []
+      ⊢ ∀P.
+            (∀m. P (m0_d m)) ∧ (∀l. P (m0u_d_stream l)) ∧
+            (∀c. P (m0u_d_word32 c)) ∧ (∀b. P (m0u_d_bool b)) ⇒
+            ∀m. P m
+   
+   [m0u_data_nchotomy]  Theorem
+      
+       []
+      ⊢ ∀mm.
+            (∃m. mm = m0_d m) ∨ (∃l. mm = m0u_d_stream l) ∨
+            (∃c. mm = m0u_d_word32 c) ∨ ∃b. mm = m0u_d_bool b
+   
+   
+*)
+end
