playground/uart_model/m0u_progTheory.sml
@@ -1,0 +1,100 @@
+structure m0u_progTheory :> m0u_progTheory =
+struct
+  
+  val _ = if !Globals.print_thy_loads
+    then TextIO.print "Loading m0u_progTheory ... "
+    else ()
+  
+  open Type Term Thm
+  local open clockTheory uartTheory in end;
+  
+  structure TDB = struct
+    val thydata = 
+      TheoryReader.load_thydata "m0u_prog"
+        (holpathdb.subst_pathvars "/home/daniil/Documents/Exjob/Kvasir/playground/uart_model/m0u_progTheory.dat")
+    fun find s = Redblackmap.find (thydata,s)
+  end
+  
+  fun op m0u_component_TY_DEF _ = ()
+  val op m0u_component_TY_DEF = TDB.find "m0u_component_TY_DEF"
+  fun op m0u_component_case_def _ = ()
+  val op m0u_component_case_def = TDB.find "m0u_component_case_def"
+  fun op m0u_component_size_def _ = ()
+  val op m0u_component_size_def = TDB.find "m0u_component_size_def"
+  fun op m0u_data_TY_DEF _ = ()
+  val op m0u_data_TY_DEF = TDB.find "m0u_data_TY_DEF"
+  fun op m0u_data_case_def _ = ()
+  val op m0u_data_case_def = TDB.find "m0u_data_case_def"
+  fun op m0u_data_size_def _ = ()
+  val op m0u_data_size_def = TDB.find "m0u_data_size_def"
+  fun op m0u_proj_def _ = () val op m0u_proj_def = TDB.find "m0u_proj_def"
+  fun op TO_M0U_def _ = () val op TO_M0U_def = TDB.find "TO_M0U_def"
+  fun op TO_M0U_PROP_def _ = ()
+  val op TO_M0U_PROP_def = TDB.find "TO_M0U_PROP_def"
+  fun op r2m0_c_set_def _ = ()
+  val op r2m0_c_set_def = TDB.find "r2m0_c_set_def"
+  fun op SDOM_def _ = () val op SDOM_def = TDB.find "SDOM_def"
+  fun op NextStateM0U_def _ = ()
+  val op NextStateM0U_def = TDB.find "NextStateM0U_def"
+  fun op M0U_MODEL_def _ = ()
+  val op M0U_MODEL_def = TDB.find "M0U_MODEL_def"
+  fun op COSIM_def _ = () val op COSIM_def = TDB.find "COSIM_def"
+  fun op datatype_m0u_component _ = ()
+  val op datatype_m0u_component = TDB.find "datatype_m0u_component"
+  fun op m0u_component_11 _ = ()
+  val op m0u_component_11 = TDB.find "m0u_component_11"
+  fun op m0u_component_distinct _ = ()
+  val op m0u_component_distinct = TDB.find "m0u_component_distinct"
+  fun op m0u_component_nchotomy _ = ()
+  val op m0u_component_nchotomy = TDB.find "m0u_component_nchotomy"
+  fun op m0u_component_Axiom _ = ()
+  val op m0u_component_Axiom = TDB.find "m0u_component_Axiom"
+  fun op m0u_component_induction _ = ()
+  val op m0u_component_induction = TDB.find "m0u_component_induction"
+  fun op m0u_component_case_cong _ = ()
+  val op m0u_component_case_cong = TDB.find "m0u_component_case_cong"
+  fun op m0u_component_case_eq _ = ()
+  val op m0u_component_case_eq = TDB.find "m0u_component_case_eq"
+  fun op datatype_m0u_data _ = ()
+  val op datatype_m0u_data = TDB.find "datatype_m0u_data"
+  fun op m0u_data_11 _ = () val op m0u_data_11 = TDB.find "m0u_data_11"
+  fun op m0u_data_distinct _ = ()
+  val op m0u_data_distinct = TDB.find "m0u_data_distinct"
+  fun op m0u_data_nchotomy _ = ()
+  val op m0u_data_nchotomy = TDB.find "m0u_data_nchotomy"
+  fun op m0u_data_Axiom _ = ()
+  val op m0u_data_Axiom = TDB.find "m0u_data_Axiom"
+  fun op m0u_data_induction _ = ()
+  val op m0u_data_induction = TDB.find "m0u_data_induction"
+  fun op m0u_data_case_cong _ = ()
+  val op m0u_data_case_cong = TDB.find "m0u_data_case_cong"
+  fun op m0u_data_case_eq _ = ()
+  val op m0u_data_case_eq = TDB.find "m0u_data_case_eq"
+  fun op NEX_thm _ = () val op NEX_thm = TDB.find "NEX_thm"
+  fun op NIT_NIT_STEP_thm _ = ()
+  val op NIT_NIT_STEP_thm = TDB.find "NIT_NIT_STEP_thm"
+  fun op NIT_COSIM_thm _ = ()
+  val op NIT_COSIM_thm = TDB.find "NIT_COSIM_thm"
+  fun op TP_def _ = () val op TP_def = TDB.find "TP_def"
+  fun op WS_COSIM_thm _ = () val op WS_COSIM_thm = TDB.find "WS_COSIM_thm"
+  
+  local open GrammarSpecials Parse
+    fun UTOFF f = Feedback.trace("Parse.unicode_trace_off_complaints",0)f
+  in
+  val m0u_prog_grammars = merge_grammars ["uart", "clock"]
+  local
+  val (tyUDs, tmUDs) = GrammarDeltas.thy_deltas{thyname="m0u_prog"}
+  val addtmUDs = term_grammar.add_deltas tmUDs
+  val addtyUDs = type_grammar.apply_deltas tyUDs
+  in
+  val m0u_prog_grammars = 
+    Portable.## (addtyUDs,addtmUDs) m0u_prog_grammars
+  val _ = Parse.grammarDB_insert("m0u_prog",m0u_prog_grammars)
+  val _ = Parse.temp_set_grammars (addtyUDs (Parse.type_grammar()), addtmUDs (Parse.term_grammar()))
+  end (* addUDs local *)
+  end
+  
+val _ = if !Globals.print_thy_loads then TextIO.print "done\n" else ()
+val _ = Theory.load_complete "m0u_prog"
+
+end
