playground/uart_model_old/decomp_experements.sml
@@ -1,0 +1,155 @@
+        
+loadPath := ("/home/daniil/HOL/examples/l3-machine-code/m0/model"::(!loadPath));
+loadPath := ("/Home/daniil/HOL/examples/l3-machine-code/common"::(!loadPath));
+loadPath := ("/home/daniil/HOL/examples/l3-machine-code/m0/decompiler"::(!loadPath));
+open  wordsTheory;
+open m0Theory;
+open m0_decompLib;
+open fcpTheory;
+
+val (code_th, code_defs) = m0_decompile "code"` 
+  00c0
+  1814
+  5ce5
+`;
+
+
+val (ldrb_th, ldrb_defs) = m0_decompile "ldrb"` 
+  5ce5
+`;
+
+val restrict_ldrb_th = prove(``! count dmem mem r3 r4 .
+SPEC M0_MODEL
+    (m0_COUNT count * m0_PC 300w * m0_MEMORY dmem mem * m0_REG RName_3 r3 *
+     m0_REG RName_4 r4 * ¬m0_REG RName_5 *
+     cond (ldrb_pre (r3,r4,count,dmem,mem) /\ r3 + r4 < 200000w) ) {(300w,INL 23781w)}
+    (let
+       (r3,r4,r5,count,dmem,mem) = ldrb (r3,r4,count,dmem,mem)
+     in
+       m0_COUNT count * m0_PC (300w + 2w) * m0_MEMORY dmem mem *
+       m0_REG RName_3 r3 * m0_REG RName_4 r4 * m0_REG RName_5 r5)
+``,			    
+let 
+ val X = DB.find "SPEC_MOVE_COND" |> List.hd|>snd|>fst 
+ val L =  Ho_Rewrite.ONCE_REWRITE_RULE [X] ldrb_th  |> GEN_ALL
+in 
+ Ho_Rewrite.REWRITE_TAC [X]>>
+ SIMP_TAC std_ss [L]
+end);
+
+decompilerLib.add_decompiled ("LDRB", SPEC_ALL restrict_ldrb_th 
+, 2, SOME 2);
+
+val (code_th, code_defs) = m0_decompile "code"` 
+00c0
+1814
+insert: LDRB
+`
+
+DB.find "SEP_IMP_REFL"
+
+``SEP_IMP (m0_COUNT count * m0_PC p * m0_MEMORY dmem mem * m0_REG RName_3 r3 *
+     m0_REG RName_4 r4 * ¬m0_REG RName_5 *
+     cond (ldrb_pre (r3,r4,count,dmem,mem)))
+
+     (m0_COUNT count * m0_PC p * m0_MEMORY dmem mem * m0_REG RName_3 r3 *
+     m0_REG RName_4 r4 * ¬m0_REG RName_5 *
+     cond (ldrb_pre (r3,r4,count,dmem,mem)))``
+EVAL_RULE code_defs
+EVAL_RULE ldrb_defs
+
+
+
+val (test2_cert, test2_def) = m0_decompile_code "test2" `
+	mov	r3, #0  		
+	lsls	r0, r0, #3 
+L:	adds	r4, r2, r0 		; r4 = key+ seq_no << 3
+	ldrb	r5, [r4, r3] 		; r5 = *(key+seq_no<<3+r3)
+	ldrb	r4, [r1, r3] 		; r4 = *(buffer+r3)
+	eors	r4, r5 			; r4 ^= r5 
+	strb	r4, [r1, r3] 		; *(buffer+r3)= r4
+	adds	r3, r3, #1 		; r3+=1
+cmp	r3, #8                  ;
+bne	L                    ; goto l10 if (r3 != 8)
+`
+val 
+
+val (test2_cert, test2_def) = m0_decompile "test2" `
+2300  
+00c0 
+1814
+5ce5  
+5ccc 
+406c 
+54cc
+3301 
+2b08 
+d1f7`
+
+
+
+val (test2_cert, test2_def) = m0_decompile "test2" `
+d1f7`
+DB.match []  ``d1f7``
+
+
+
+val (test2_cert, test2_def) = m0_decompile_code "test2" `
+cmp	r3, #8                  ;
+bne	L                    ; goto l10 if (r3 != 8)
+`
+
+
+
+
+
+
+val n = prove(``!r0 r1 r2 r3 count dmem mem.
+  (test21 (r0,r1,r2,r3,count,dmem,mem) =
+   if r3 + 1w = 8w then
+     (r0,r1,r2,r3 + 1w,w2w (mem (r1 + r3)) ⊕ w2w (mem (r2 + r0 + r3)),
+      w2w (mem (r2 + r0 + r3)),count + 1 + 2 + 2 + 1 + 2 + 1 + 1 + 1,
+      dmem,
+      (r1 + r3 =+
+       (7 >< 0) (w2w (mem (r1 + r3)) ⊕ w2w (mem (r2 + r0 + r3)))) mem)
+   else
+     test21
+       (r0,r1,r2,r3 + 1w,count + 1 + 2 + 2 + 1 + 2 + 1 + 1 + 3,dmem,
+        (r1 + r3 =+
+         (7 >< 0) (w2w (mem (r1 + r3)) ⊕ w2w (mem (r2 + r0 + r3))))
+          mem))``,
+	  
+SIMP_TAC arithm_ss []
+EVAL_TAC
+
+)
+
+
+``!r0 r1 r2 r3 count dmem mem.
+  (test21 (r0,r1,r2,r3,count,dmem,mem) =
+  (r0, r1, r2, 8w,
+   w2w (mem (r1 + 8w)) ⊕ w2w (mem (r2 + r0 + 8w)),
+   w2w (mem (r2 + r0 + 8w)),
+  count+11* w2n(8w-r3),
+  dmem,
+  \a.  if r1 +r3 <= a /\ a <= r1+8w
+       then (7 >< 0) (w2w (mem a) ⊕ w2w (mem (r2 + r0 + (a-r1))))
+       else mem a))
+       
+``
+REPEAT STRIP_TAC
+Induct_on `w2n (8w - r3)`
+
+`r3 = 7w` by 
+DB.match
+DB.match [] ``_/\ (∀n. P _ ⇒ P _) ⇒ ∀n. P _``
+DB.find  "induct"
+EVAL_TAC
+
+ONCE_REWRITE_TAC [test2_def]
+EVAL_TAC
+
+
+DB.find "while"
+EVAL_TAC
+
