playground/uart_model/m0u_progScript.sml
@@ -1,13 +1,14 @@
 open HolKernel Parse boolLib bossLib;
-open uartTheory
-open progTheory 
-open set_sepTheory
-open m0_NITTheory
-open uartTheory
-open clockTheory
-open stateTheory m0_stepTheory
-open boolSimps
-open pred_setTheory
+open uartTheory;
+open progTheory;
+open set_sepTheory;
+open m0_NITTheory;
+open m0_progTheory;
+open uartTheory;
+open clockTheory;
+open stateTheory m0_stepTheory;
+open boolSimps;
+open pred_setTheory;
 
 val _ = new_theory "m0u_prog";
 (********************************************)
@@ -62,23 +63,79 @@ r2m0_c_set region = IMAGE m0_c_MEM region
 val m0_SDOM_def = Define`
 SDOM A = (BIGUNION (IMAGE (IMAGE (\(c,_).c)) A)) `;
 
+
+``DISJOINT (SDOM (m0_count 3 * m0_REG )) (r2m0_c_set uart_r)``
+SIMP_TAC (std_ss++pred_setLib.PRED_SET_ss) [m0_count_def, m0_SDOM_def, r2m0_c_set_def, m0_component_distinct]
+DB.find "m0_REG"
+
 val m0_SEP_INV_UNDER_NON_R_EQ_thm = prove(
 ``!P region s s'. DISJOINT (SDOM P) (r2m0_c_set region) 
     /\ SEP_REFINE (P * SEP_T) $= (STATE m0_proj) s 
     /\ m0_non_r_eq region s s' ==>
 	SEP_REFINE (P * SEP_T) $= (STATE m0_proj) s'``,
-cheat);
+ASM_SIMP_TAC (std_ss++pred_setLib.PRED_SET_ss) [PULL_EXISTS, SEP_REFINE_def, STATE_def, STAR_def, SPLIT_def]
+	     REPEAT STRIP_TAC
+	    Q.EXISTS `u` 
+	     
+	     DB.find "STAR"
+	     DB.find "SPLIT_def"
+	     
+	     DB.find "SUBSET_EQ"
+	     
+
+val disjoint_thm = prove(``!s s' m  region.
+DISJOINT (SDOM P) (r2m0_c_set region) 
+    /\ P m ==>
+ m SUBSET( COMPL(r2m0_c_set region))``)
+
+ /\
+ m0_non_r_eq region s s' ==>
+ SEP_REFINE (P ) $= (STATE m0_proj) s
+    ((SELECT_STATE m0_proj m s) =(SELECT_STATE m0_proj m s'))``, 
+SIMP_TAC std_ss [FUN_EQ_THM]>>
+REPEAT STRIP_TAC>>
+Cases_on `x`>>
+FULL_SIMP_TAC (std_ss++pred_setLib.PRED_SET_ss) [
+    FRAME_STATE_def, SELECT_STATE_def,
+    fun2set_def, m0_non_r_eq_def, m0_proj_def, 
+    r2m0_c_set_def,m0_component_distinct, mem_eq_def]>>
+Cases_on `q`>>
+    FULL_SIMP_TAC (std_ss++pred_setLib.PRED_SET_ss) [ SUBSET_DEF, m0_component_case_def, m0_component_11, m0_data_11]>>
+
+    METIS_TAC[]
+);
+
+
+
+val m0_nen_eq_state_set_eq_thm = prove(``!s s' m  region.
+ m SUBSET( COMPL(r2m0_c_set region)) /\
+ m0_non_r_eq region s s' ==>
+    ((SELECT_STATE m0_proj m s) =(SELECT_STATE m0_proj m s'))``, 
+SIMP_TAC std_ss [FUN_EQ_THM]>>
+REPEAT STRIP_TAC>>
+Cases_on `x`>>
+FULL_SIMP_TAC (std_ss++pred_setLib.PRED_SET_ss) [
+    FRAME_STATE_def, SELECT_STATE_def,
+    fun2set_def, m0_non_r_eq_def, m0_proj_def, 
+    r2m0_c_set_def,m0_component_distinct, mem_eq_def]>>
+Cases_on `q`>>
+    FULL_SIMP_TAC (std_ss++pred_setLib.PRED_SET_ss) [ SUBSET_DEF, m0_component_case_def, m0_component_11, m0_data_11]>>
+
+    METIS_TAC[]
+);
+
 
 (********************************************)
 (*          Uart model prog                 *)
 (*                                          *)
 (********************************************)
-val NextStateM0U_def = Define ` NextStateM0U ((s0,u0),I0,O0) =
+
+val NextStateM0U_def = Define ` NextStateM0U s0 =
       (let
-        ((s1,u1),I1,O1)  = m0u_Next ((s0,u0),I0,O0)
+        s1  = m0u_Next s0
       in
-          if (~u1.unpredictable /\ (s1.exception = NoException))
-         then SOME ((s1,u1),I1,O1) else NONE)`;
+          if (~(((SND o FST)s1).unpredictable) /\ (((FST o FST)s1).exception = NoException))
+         then SOME s1 else NONE)`;
 
 val M0U_MODEL = Define `M0U_MODEL = (
     STATE m0u_proj,
@@ -92,104 +149,163 @@ val COSIM_def = Define ` COSIM P t = ! s s' seq seq' i.
     ((SEP_REFINE (P * SEP_T) ($=) (STATE m0_proj) s) /\
     rel_sequence (NEXT_REL $= NextStateM0) seq  s /\
     rel_sequence (NEXT_REL $= NextStateM0U) seq' s' /\
+    ~(((SND o FST) s').unpredictable)/\
     m0u_m0_non_r_eq uart_r s' s /\ ((seq i).count <= s.count + t) )==>   
 	m0u_m0_non_r_eq uart_r (seq' i) (seq i) /\
 	m0u_r_eq uart_r s' (seq' i)`;
 
-
-val m0_non_r_eq_exists_thm = prove(``!s region.?s'. m0_non_r_eq region s s'``,
-     METIS_TAC [m0_non_r_eq_refl_thm]
+val NEX_thm = Q.store_thm("NEX_thm",
+    `! P t s seq i.
+	NEX P t ==> (
+	    SEP_REFINE (P * SEP_T) $= (STATE m0_proj) s /\
+	    rel_sequence (NEXT_REL $= NextStateM0) seq s /\
+	    (seq (SUC i)).count <= s.count + t ==> 
+                ((seq i).count < (Next(seq i)).count) /\ ((Next (seq i)) = (seq(SUC i))))`,
+    REPEAT STRIP_TAC>>
+    FULL_SIMP_TAC (std_ss++LET_ss) [NEX_def, PULL_FORALL]>>
+    Q.PAT_X_ASSUM `!s seq i._` (MP_TAC o Q.SPECL [`s`,`seq`, `i`])>>
+    FULL_SIMP_TAC (std_ss++LET_ss) [NEX_def, PULL_FORALL,rel_sequence_def, 
+			    NEXT_REL_EQ, NextStateM0_def]>>
+    METIS_TAC[]
 );
 
-   (** third attempt with stronger induction assumption **) 
+
+
+val PRODUCT_STATE_lem = prove(``!s z_i. ?z_0. m0_non_r_eq uart_r s z_0 /\ m0_r_eq uart_r z_0 z_i``,
+    REPEAT GEN_TAC>>
+    EXISTS_TAC ``s with <|MEM := (\x. if (x IN uart_r) 
+                                         then (z_i.MEM x)
+                                         else (s.MEM x)) |>``>>
+    SIMP_TAC (std_ss++pred_setLib.PRED_SET_ss) [m0Theory.m0_state_accfupds,
+		m0_non_r_eq_def, m0_r_eq_def, mem_eq_def]
+);
+
+val eq_lem = prove(``!a b r.
+    m0_non_r_eq r a  b /\ m0_r_eq r a b ==> (a=b)``,
+			      
+    REPEAT GEN_TAC>>
+    Cases_on `a`>>Cases_on `b`>>
+    SIMP_TAC (std_ss++pred_setLib.PRED_SET_ss) [m0Theory.m0_state_accfupds,
+m0Theory.m0_state_accessors,m0_non_r_eq_def, m0_r_eq_def, mem_eq_def, m0Theory.m0_state_11]>>
+    Cases_on  `x NOTIN r ` >> METIS_TAC[]
+);
+
+val   NIT_NIT_STEP_thm = store_thm("NIT_NIT_STEP_thm",
+``  ! P t s seq i.
+	NIT uart_r P t /\
+	NEX P t ==> (
+	SEP_REFINE (P * SEP_T) $= (STATE m0_proj) s /\
+	rel_sequence (NEXT_REL $= NextStateM0) seq s /\
+	(seq (SUC i)).count <= s.count + t ==> NIT_STEP uart_r (seq i))``,
+    REPEAT STRIP_TAC >>
+    SIMP_TAC std_ss [NIT_STEP_thm]>>
+    GEN_TAC>>
+    rename1 `m0_non_r_eq uart_r (seq i) z_i`>>
+    STRIP_TAC>>
+    `?z_0. m0_non_r_eq uart_r s z_0 /\ m0_r_eq uart_r z_0 z_i` by( 
+        METIS_TAC[PRODUCT_STATE_lem]
+    )>>
+    `?seq_z . rel_sequence (NEXT_REL $= NextStateM0) seq_z z_0` by(
+        METIS_TAC[SEQUENCE_EXISTS_THM]
+    )>>
+ 
+    `(seq i).count ≤ s.count + t` by(
+	METIS_TAC[NEX_thm,
+	    DECIDE ``((a:num) < (b:num) /\ b <= (c:num)) ==>( a <= c)``])>>
+
+    `z_i = seq_z i ` by (
+	Q.PAT_ASSUM `NIT uart_r P t` (MP_TAC o 
+				  Q.SPECL [`s`, `z_0`, `seq`, `seq_z`, `i`] o
+                                  REWRITE_RULE [NIT_def])>>
+	METIS_TAC[m0_r_eq_trans_thm, m0_r_eq_antisym_thm,
+                  m0_non_r_eq_trans_thm, m0_non_r_eq_antisym_thm,
+                  eq_lem])>>
+    
+    Q.PAT_ASSUM `NIT uart_r P t` (MP_TAC o 
+	   			  Q.SPECL [`s`, `z_0`, `seq`, `seq_z`, `SUC i`] o
+                                  REWRITE_RULE [NIT_def])>>
+    ASM_SIMP_TAC std_ss []>>
+    STRIP_TAC>>
+
+    `(seq(SUC i) = Next (seq(i)))` by  (METIS_TAC[NEX_thm])>>
+
+   `(seq_z(SUC i) = Next (seq_z(i)))` by(
+        (* a step must have taken place between (seq_z i) and i+1 
+           since the count between them has increesed *) 
+	`(seq_z(i)).count < (seq_z(SUC i)).count ` by
+	    METIS_TAC[NEX_thm,  m0_non_r_eq_def]>>
+	Q.PAT_X_ASSUM `rel_sequence (NEXT_REL $= NextStateM0) seq_z s_0` 
+	    (MP_TAC o Q.SPEC `i` o 
+	    SIMP_RULE (std_ss++LET_ss)[
+		rel_sequence_def, PULL_EXISTS,NEXT_REL_EQ,
+		NextStateM0_def, PULL_FORALL])>>
+         IF_CASES_TAC >-  (METIS_TAC[] )>>
+	 STRIP_TAC >> FULL_SIMP_TAC arith_ss[]
+    )>>
+    
+    METIS_TAC[m0_r_eq_trans_thm,m0_r_eq_antisym_thm]
+);
+ 
+val LEM = prove(
+    ``!(a:((m0_state # uart_state) # word32 list # word32 list)) 
+       (b:((m0_state # uart_state) # word32 list # word32 list)) region.
+	    m0u_r_eq region a b ==> ((SND (FST a)) = (SND (FST b)))``, 
+    Cases_on `a`>> Cases_on `b`>> Cases_on `q`>>
+    Cases_on `q'`>> Cases_on `r`>> Cases_on `r'`>>
+    SIMP_TAC std_ss [m0u_r_eq_def]
+);
+val LEM1 = prove(
+    ``!a b region. (m0u_m0_non_r_eq  region a b) ==> 
+	((FST (FST a)).count =  b.count)/\
+	((FST (FST a)).exception =  b.exception)``, 
+    Cases_on `a`>> Cases_on `q`>> Cases_on `r`>>
+    SIMP_TAC std_ss [m0u_m0_non_r_eq_def, m0_non_r_eq_def]
+);
+
 val NIT_COSIM_thm = Q.store_thm ("NIT_COSIM_thm", 
     `!P t.  ((NIT uart_r P t) /\ (NEX P t)) ==> (COSIM P t)`, 
     SIMP_TAC std_ss [ COSIM_def, PULL_FORALL]>>
-    (* Strengthen induction hypothesis  *)
-    `!P t s s' s_hat seq seq'  seq_hat i .
-        (m0_non_r_eq uart_r s s') /\
-	NIT uart_r P t /\
-	NEX P t ==>
-	SEP_REFINE (P * SEP_T) $= (STATE m0_proj) s /\
-	rel_sequence (NEXT_REL $= NextStateM0) seq s /\
-	rel_sequence (NEXT_REL $= NextStateM0) seq' s' /\
-	rel_sequence (NEXT_REL $= NextStateM0U) seq_hat s_hat /\
-	m0u_m0_non_r_eq uart_r s_hat s /\ (seq i).count <= s.count + t ==>
-        m0_non_r_eq uart_r (seq i) (seq' i) /\
-        m0_r_eq uart_r s' (seq' i) /\
-	m0u_m0_non_r_eq uart_r (seq_hat i) (seq i) /\
-	m0u_r_eq uart_r s_hat (seq_hat i) ` suffices_by(
-            METIS_TAC [m0_non_r_eq_exists_thm, SEQUENCE_EXISTS_THM]
-    )>>
     REPEAT GEN_TAC>>
-    Induct_on `i`>-(   
-        `s.count <= s.count +t` by DECIDE_TAC>>
-	METIS_TAC [m0u_m0_non_r_eq_def, m0u_r_eq_refl_thm,
-                   m0_r_eq_refl_thm , rel_sequence_def]
+    Induct_on `i`>-(
+        ASM_SIMP_TAC std_ss [rel_sequence_def, m0u_r_eq_refl_thm]
     )>>
     STRIP_TAC>>STRIP_TAC>>
-    `(seq i).count <= s.count + t ` by (
-	(MP_TAC o Q.SPECL [`s`,`i`, `SUC i`, `seq`]) SEQ_MONO_B >>
-	ASM_SIMP_TAC std_ss []>>
-	DECIDE_TAC)>>
+
+    `(seq i).count ≤ s.count + t` by(
+	METIS_TAC[NEX_thm,
+	    DECIDE ``((a:num) < (b:num) /\ b <= (c:num)) ==>( a <= c)``])>>
     FULL_SIMP_TAC std_ss []>>
-    
-    Q.PAT_ASSUM `NIT uart_r _ _` (MP_TAC o Q.SPECL [`s`, `s'`, `seq`, `seq'`, `SUC i`]
-                                           o SIMP_RULE std_ss [ NIT_def])>>
-    FULL_SIMP_TAC std_ss []>>
-    STRIP_TAC >>
+    (MP_TAC o Q.SPECL [`P`,`t`,`s`,`seq`, `i`]) NIT_NIT_STEP_thm>>
+    ASM_SIMP_TAC std_ss[]>>
+    STRIP_TAC>>
+    `(seq(SUC i) = Next (seq(i)))` by  (METIS_TAC[NEX_thm])>>
+    (MP_TAC o Q.SPECL [`seq (i:num)`, `seq' (i:num)`]) AXI>>
+    ASM_SIMP_TAC std_ss[]>>
+    STRIP_TAC>>
 
-    (* should get from from NEX: *)
-
-     `(seq(SUC i) = Next (seq(i))) /\ ((Next (seq i)).exception = NoException)` by (
-	Q.PAT_X_ASSUM `NIX P t` (
-            MP_TAC o Q.SPECL [`s`, `seq`, `SUC i`] o
-	    REWRITE_RULE [NEX_def])>>
-	FULL_SIMP_TAC (std_ss++LET_ss) [
-	    rel_sequence_def, NEXT_REL_EQ,
-            NextStateM0_def]>>
-        METIS_TAC []  
-      )>>
-   
-      
-
-    `(seq'(SUC i) = Next (seq'(i))) ` by(
-     `((seq' (SUC i)).exception = NoException)` by  FULL_SIMP_TAC std_ss[m0_non_r_eq_def]>>
-	FULL_SIMP_TAC (std_ss++LET_ss) [
-	    rel_sequence_def, NEXT_REL_EQ,
-            NextStateM0_def]>>
-	Cases_on  `(Next (seq' i)).exception = NoException`>- (
-	    METIS_TAC [])>>
-	Q.PAT_ASSUM `!n.
-		if (Next (seq' n)).exception = NoException then
-		    Next (seq' n) = seq' (SUC n)
-		else seq' (SUC n) = seq' n` (MP_TAC o Q.SPECL [`i`])>>
-	`(seq i).count = (Next(seq i)).count` suffices_by (
-	    (MP_TAC o Q.SPEC `seq (i:num)`) NEXT_MONO>>
-	    ASM_SIMP_TAC arith_ss [])>>
-	FULL_SIMP_TAC std_ss [m0_non_r_eq_def] >>
-	METIS_TAC[]
+    `seq' (SUC i) = m0u_Next (seq' i)` by (
+	`(Next (seq i)).exception = NoException` by (
+	    Q.PAT_X_ASSUM `NIX P t` ( 
+                MP_TAC o Q.SPECL [`s`, `seq`, `i`] o
+		REWRITE_RULE [NEX_def])>>
+	    FULL_SIMP_TAC std_ss []
+	)>>
+	` m0u_r_eq uart_r s' (m0u_Next (seq' i))` by(
+	    METIS_TAC [m0u_r_eq_trans_thm, m0u_r_eq_antisym_thm]
+        )>>
+	Q.PAT_X_ASSUM `rel_sequence (NEXT_REL $= NextStateM0U) seq' s'` (MP_TAC o
+	    SPEC ``i:num`` o
+	    CONJUNCT2 o
+	    REWRITE_RULE [PULL_FORALL,rel_sequence_def, 
+                          NEXT_REL_EQ, NextStateM0U_def]
+            
+        )>>
+	ASM_SIMP_TAC (std_ss++LET_ss) []>>
+	METIS_TAC[NextStateM0U_def, LEM, LEM1]
     )>>
-    FULL_SIMP_TAC std_ss []>>
-
-    (* from NIT_STEP_thm and 16, 12, 13 *)
-    `NIT_STEP uart_r (seq i)`  suffices_by cheat
-    
-    ASM_SIMP_TAC std_ss  [NIT_STEP_thm, m0_non_r_eq_antisym_thm, m0_non_r_eq_trans_thm, m0_r_eq_trans_thm, m0_r_eq_antisym_thm]
-    
-    DB.find "NIT_STEP_thm"
-    SIMP_RULE std_ss [PULL_FORALL] NIT_STEP_thm
-    
-    (MP_TAC o Q.SPECL [`seq (i:num)`, `seq_hat (i:num)`]) AXI>>
-    ASM_SIMP_TAC std_ss [NIT_STEP_def, NIT_STEP_from_def]>> 
-DB.find "NIT_STEP_from"
-    
-    (* uart does not change, so uart is still predictable *)
-    `seq_hat(SUC i) = m0u_Next (seq_hat i)` by cheat>>
     METIS_TAC [m0u_r_eq_trans_thm,  m0u_r_eq_antisym_thm]
 );
 
-    
 
 (********************************************)
 (*          Transfere properties            *)
@@ -202,9 +318,7 @@ val TP_def = Q.store_thm(
     "TP_def",
     `!P C Q c t. (SPEC M0_MODEL (P*m0_count c) C (Q*m0_count (c+t))) /\ 
 	(COSIM P t) /\  
-
-(!SET. P SET==>  DISJOINT SET UART) /\
-(!SET. Q SET==>  DISJOINT SET UART) ==>
+    (!SET. P SET==>  DISJOINT SET UART) /\ (!SET. Q SET==>  DISJOINT SET UART) ==>
 
  
 	    (SPEC M0U_MODEL (TO_M0U_PROP (P*m0_count c)) C (TO_M0U_PROP(Q*m0_count (c+t))))`,
@@ -214,10 +328,10 @@ val WS_COSIM_thm = Q.store_thm("WS_COSIM_thm",
     `!P P' t t'. COSIM P t /\ t' < t  /\ (SEP_IMP P' P) ==> COSIM P' t'`,
     SIMP_TAC arith_ss [COSIM_def, PULL_FORALL]>>
     REPEAT STRIP_TAC>>(
-	Q.PAT_X_ASSUM `!s s' seq seq' i F._` (MP_TAC o Q.SPECL [`s`, `s'`, `seq`, `seq'`, `i`, `F'`] )>>
+	Q.PAT_X_ASSUM `!s s' seq seq' i._` (MP_TAC o Q.SPECL [`s`, `s'`, `seq`, `seq'`, `i`] )>>
 	REPEAT STRIP_TAC>>
-	` (seq i).count ≤ t` by DECIDE_TAC>>
-	`SEP_REFINE (P * F') $= (STATE m0_proj) s` by (
+	` (seq i).count ≤ t+s.count` by DECIDE_TAC>>
+	`SEP_REFINE (P * SEP_T) $= (STATE m0_proj) s` by (
 	REV_FULL_SIMP_TAC std_ss [SEP_IMP_def, STAR_def,SEP_REFINE_def]>>
 	METIS_TAC [])>>
 	METIS_TAC []
