playground/uart_model_old/uartScript.sml
@@ -1,26 +1,44 @@
-open HolKernel Parse boolLib;
-open boolSimps;
-open bossLib;
-open wordsTheory;
+loadPath := ("/home/daniil/HOL/examples/l3-machine-code/m0/model"::(!loadPath));
+loadPath := ("/Home/daniil/HOL/examples/l3-machine-code/common"::(!loadPath));
+loadPath := ("/home/daniil/HOL/examples/l3-machine-code/m0/decompiler"::(!loadPath));
+open  wordsTheory;
 open m0Theory;
+open m0_decompLib;
 open fcpTheory;
-open m0_NITTheory;
 
-val _ = new_theory "uart";
+
+val _ = new_theory "uartModel";
+
+(*
+
+DB.find "Next"
+DB.find "SEP_REFINE_def"
+DB.find "SPEC_def"
+DB.find "m0_MODEL"
+
+DB.find  "STATE_def"
+DB.find  "CODE_POOL"
+DB.find  "m0_instr"
+
+DB.match ["m0_prog"] ``_``
+
+DB.find "m0_state_typedef"
+DB.find "m0_state_induct"
+*)
+
 
 (*********************************)
 (*   buffer model                *)
 (*********************************)
-
 val _= Datatype `buffer = <| data: word32 ['n];
                               h:num;
                               t:num;
-                              Size:num;
+                              size:num;
                               cap:num; |>`;
 
 val bufferN_def = Define `
 Buffer (:'n) = <| data := (FCP i. 0w):word32['n];
-                  h:=0; t:=0; Size:= 0;
+                  h:=0; t:=0; size:= 0;
                   cap:=dimindex(:'n); |>`;
 
 val Pop_def = Define `
@@ -28,15 +46,28 @@ Pop  buf =  ((* Result: *)
                 (buf.data ' buf.t),
              (* Next  buffer state:*) 
                 (buf with <|  t updated_by SUC;  
-                                   Size updated_by PRE|>))`;
+                                   size updated_by PRE|>))`;
 
 val Push_def = Define `
 Push el buf  =  buf with <| data updated_by ( (buf.h MOD buf.cap) :+ el);
                             h    updated_by SUC ;
-                            Size updated_by  SUC ;|>
+                            size updated_by  SUC ;|>
 `;
 
-val  _ = EVAL ``     Buffer (:5)   :> (Push 1w)
+val option_fapply2 = Define `
+((ofap f  NONE) = NONE) /\
+((ofap f (SOME x)) = (f x))
+`;
+
+val option_fapply2 = Define `
+((A f (out0, NONE)) = (out0,NONE)) /\
+((A f (out0, SOME x)) = let
+    (out1, next) = f x;
+in if out1 = NONE 
+   then  (out0, next)
+   else  ([THE out1] ++ out0, next))  `;
+
+EVAL ``     Buffer (:5)   :> (Push 1w)
                           :> (Push 2w)
                           :> (Push 3w)
                           :> (Push 4w)
@@ -44,14 +75,15 @@ val  _ = EVAL ``     Buffer (:5)   :> (Push 1w)
                           :> (Push 6w)
                           :> Pop
                           :> \(x,y). y
-                          :> Pop``;
+                          :> Pop``
+
+val option_testbuffer = Define  `testbuf= <| data:=[0w;1w;2w;3w];cap:=6|>`;
 
 (***********************************************)
 (*      uart                                   *)
 (***********************************************)
 
 val _= Datatype `uart_state = <|enabled: bool; 
-				unpredictable:bool;
 		                rx_started: bool; 
                                 tx_started:bool;
                                 RXD: word32;
@@ -60,7 +92,7 @@ val _= Datatype `uart_state = <|enabled: bool;
 				TXDRDY: bool;
                                 PINSELRXD: word32;
                                 PINSELTXD:word32;
-                                RBUF:6 buffer ;
+                                RBUF:'n buffer ;
                                 transmit: bool;
                                 rxd_cleared: bool;
                                 |>`;
@@ -207,8 +239,7 @@ val _= Datatype `uart_mmap = <|
 *)
 
 val nRF51_uart_initial_state_def   = Define`
-    nRF51_uart_initial_state = <|
-        unpredictable:=F;
+    nRF51_uart_initial_state = <|   
 	enabled:= F; 
 	rx_started:= F; 
 	tx_started:= F;
@@ -223,7 +254,7 @@ val nRF51_uart_initial_state_def   = Define`
         rxd_cleared:=F;
 |>`;
 
-(*
+
 val uart_pop_rbuf_def = Define `
  uart_pop_rbuf uart =
  let
@@ -243,154 +274,6 @@ val uart_push_rbuf_def = Define `
     then  (NONE, NONE)
     else  (r, SOME( uart with RBUF updated_by (\x. THE n)))
 `;
-*)
-
-
-(*******************************************)
-(*          UART NIF                       *)
-(*******************************************)
-     
-val m0u_r_eq_def = Define `
-    m0u_r_eq region ((s1,u1),in1,out1) ((s2, u2),in2,out2)  = 
-        m0_r_eq region s1 s2 /\ (u1=u2) /\ (out1=out2) /\ (in1=in2)`;
-
-val m0u_non_r_eq_def = Define `
-    m0u_non_r_eq region ((s1,u1),in1,out1) ((s2, u2),in2,out2) = 
-        m0_non_r_eq region s1 s2`;
-
-val m0u_m0_non_r_eq_def = Define `
-    m0u_m0_non_r_eq region ((s1,u1),in1,out1) s2 = 
-        m0_non_r_eq region s1 s2`;
-
-val m0u_r_eq_refl_thm = Q.store_thm("m0u_r_eq_refl_thm",
-`!region s. m0u_r_eq region s s`,
-
-    Cases_on `s`>>
-    Cases_on `r`>>
-    Cases_on `q`>>
-    METIS_TAC[m0u_r_eq_def, m0_r_eq_refl_thm]
-);
-
-val m0u_non_r_eq_refl_thm = Q.store_thm("m0u_non_r_eq_refl_thm",
-`!region s. m0u_non_r_eq region s s`,
-
-    Cases_on `s`>>
-    Cases_on `r`>>
-    Cases_on `q`>>
-    METIS_TAC[m0u_non_r_eq_def, m0_non_r_eq_refl_thm]
-);
-
-val m0u_r_eq_antisym_thm = Q.store_thm("m0u_r_eq_antisym_thm",
-    `!region s1 s2. m0u_r_eq region s1 s2 = m0u_r_eq region s2 s1`,
-    Cases_on `s1`>>
-    Cases_on `s2`>>
-    Cases_on `r`>>
-    Cases_on `r'`>>
-    Cases_on `q`>>
-    Cases_on `q'`>>
-    METIS_TAC[m0u_r_eq_def, m0_r_eq_antisym_thm]
-);
-
-val m0u_non_r_eq_antisym_thm = Q.store_thm("m0u_non_r_eq_antisym_thm",
-    `!region s1 s2. m0u_non_r_eq region s1 s2 = m0u_non_r_eq region s2 s1`,
-    Cases_on `s1`>>
-    Cases_on `s2`>>
-    Cases_on `r`>>
-    Cases_on `r'`>>
-    Cases_on `q`>>
-    Cases_on `q'`>>
-    METIS_TAC[m0u_non_r_eq_def, m0_non_r_eq_antisym_thm]);
-
-val m0u_r_eq_trans_thm = Q.store_thm("m0u_r_eq_trans_thm",
-    `!region s1 s2 s3. m0u_r_eq region s1 s2 /\ m0u_r_eq region s2 s3 ==> m0u_r_eq region s1 s3`,
-    Cases_on `s1`>>
-    Cases_on `s2`>>
-    Cases_on `s3`>>
-    Cases_on `q`>>
-    Cases_on `q'`>>
-    Cases_on `q''`>>
-    Cases_on `r`>>
-    Cases_on `r'`>>
-    Cases_on `r''`>>
-    METIS_TAC[m0u_r_eq_def, m0_r_eq_trans_thm]
-);
-
-val m0u_non_r_eq_trans_thm = Q.store_thm("m0u_non_r_eq_trans_thm",
-    `!region s1 s2 s3. m0u_non_r_eq region s1 s2 /\ m0u_non_r_eq region s2 s3 ==> m0u_non_r_eq region s1 s3`,
-    Cases_on `s1`>>
-    Cases_on `s2`>>
-    Cases_on `s3`>>
-    Cases_on `q`>>
-    Cases_on `q'`>>
-    Cases_on `q''`>>
-    Cases_on `r`>>
-    Cases_on `r'`>>
-    Cases_on `r''`>>
-    METIS_TAC[m0u_non_r_eq_def, m0_non_r_eq_trans_thm]);
-
-val ward_region_def = Define`
-(* TODO: change to bit masking? *)
-ward_region (x:word32) = {x;x+1w; x+2w;x+3w}
-`;
-
-val uart_r_def = Define`
-uart_r=(ward_region(nRF51_uart_mmap STARTRX) UNION
-ward_region(nRF51_uart_mmap STOPRX) UNION
-ward_region(nRF51_uart_mmap STARTTX) UNION
-ward_region(nRF51_uart_mmap STOPTX) UNION
-ward_region(nRF51_uart_mmap SUSPEND) UNION
-ward_region(nRF51_uart_mmap CTS) UNION
-ward_region(nRF51_uart_mmap NCTS) UNION
-ward_region(nRF51_uart_mmap RXDRDY) UNION
-ward_region(nRF51_uart_mmap TXDRDY) UNION
-ward_region(nRF51_uart_mmap ERROR) UNION
-ward_region(nRF51_uart_mmap RXTO) UNION
-ward_region(nRF51_uart_mmap INTEN) UNION
-ward_region(nRF51_uart_mmap INTENSET) UNION
-ward_region(nRF51_uart_mmap INTENCLR) UNION
-ward_region(nRF51_uart_mmap ERRORSRC) UNION
-ward_region(nRF51_uart_mmap ENABLE) UNION
-ward_region(nRF51_uart_mmap PSELRTS) UNION
-ward_region(nRF51_uart_mmap PSELTXD) UNION
-ward_region(nRF51_uart_mmap PSELCTS) UNION
-ward_region(nRF51_uart_mmap PSELRXD) UNION
-ward_region(nRF51_uart_mmap RXD) UNION
-ward_region(nRF51_uart_mmap TXD) UNION
-ward_region(nRF51_uart_mmap BAUDRATE) UNION
-ward_region(nRF51_uart_mmap CONFIG))`
-
-
-
-(*
-this theorem does not hold sincethere are gaps in uart registers right now 
-
-``uart_r = {addr| addr >= 0x40002000w /\ addr <= (0x4000256Cw+3w)}``
-
-
-ASM_SIMP_TAC (arith_ss++pred_setLib.PRED_SET_ss++wordsLib.WORD_LOGIC_ss  ) [FUN_EQ_THM, uart_r_def, ward_region_def, nRF51_uart_mmap_def] 
-
-
-REPEAT STRIP_TAC>>
-
-
-val tactic1 = (fn x => 
-Cases_on (`x:word32 = `@[QUOTE ((Int.toString x)^"w:word32")])
->- (ASM_SIMP_TAC std_ss []>> blastLib.FULL_BBLAST_TAC )
-)
-fun tactical1 a b = if a=b 
-    then tactic1 a >> (PAT_X_ASSUM ``_`` MP_TAC) 
-    else (tactic1 a >> 
-          (PAT_X_ASSUM ``_`` MP_TAC) >>
-          (tactical1 (a+1) b))		   
-
-tactical1 (0x40002000) (0x4000200f)
-
-*)
-
-
-(*******************************************)
-(*          NEXT function                  *)
-(*******************************************)
 
 val uart_next_cpu_def = Define`
     uart_next_cpu event uart = 
@@ -458,7 +341,7 @@ val uart_next_cpu_def = Define`
 		   |LOAD w CONFIG => NONE
 `;
 
-(*
+
 uart_next_io_def = Define `
     uart_next_io (input:word32 option) uart =
         case input of 
@@ -469,50 +352,266 @@ uart_next_io_def = Define `
                     else (NONE, uart)   
           | SOME w => (NONE, uart)
 
-)`;
-*)
+)`
 
-val m0u_Next_def= Define 
-`m0u_Next (((s:m0_state), (u:uart_state)), (input:word32 list), (output:word32 list)) =  
-    if NIT_STEP uart_r s
-    then     ((Next s,u) ,input, output)
-    else  
-(*** IMPLEMENT the actual model
+
+(* TODO *)
+val load_uart_register_def = Define`
+load_uart_register uart reg (cpu:m0_state) = cpu
+`;
+
+(* TODO *)
+val addres_def = Define`
+addres n m state = let 
+    (v,s) = case m of
+                immediate_form imm32 => (imm32, state)
+              | register_form m =>
+                  Shift (R m state,SRType_LSL,0,state.PSR.C) state 
+
+(** Model definition using Fetch-Decode to detect transition type  **)
+(* TODO: finissh definiton *)
+val cpu_next_def Define`
+   cpu_next cpu uart = in
+     ( v, s ) = Fetch cpu;
+     ( v, s ) = Decode v s;
+   let case s of
+     Load  (LoadWord  ( t, n, m)) => case nRF51_uart_mmap' (addres n m cpu) of
+                                        NONE => ( SOME (next cpu), SOME uart )
+                                        SOME reg =>  ( (* load cpu register*) SOME (next cpu ), uart_next_cpu (LOAD reg) uart )
+
+     Store (StoreWord ( t, n, m)) => case nRF51_uart_mmap' (addres n m cpu) of
+                                        NONE => ( SOME (next cpu), SOME uart )
+                                        SOME reg =>  ( SOME (next cpu ), uart_next_cpu (STORE reg) uart )
+     Data a => (SUME (next cpu), SEME uart) 
+     w => (NONE, NONE) 
+`;
+
+(** Model using information flow to detect transition type **)
+
+val is_uart_reg_addr_def = Define`
+(* TODO: change to bit masking? *)
+is_uart_reg_addr (addr:'a word) = (addr >= 0x40002000w /\ addr <= 0x4000256Cw)
+`;
+
+(*
+val load_uart_reg_def = Define `
+load_uart_reg s = let
+    ( v, s) = Fetch s;
+    ( v, s) = Decode v s;
+in ?t n m. (v  = Load  (LoadWord  ( t, n, m))) /\
+    ( is_uart_reg_addr (addres n m s) )
+(* TODO: extend to cover other loads eg load type *)
+`;
+
+
+val load_uart_reg2_def = Define `
+(*not sure if cases or exists is better*)
+load_uart_reg2 s = let
+    ( v, s) = Fetch s;
+    ( v, s) = Decode v s;
+in case v of 
+    (Load  (LoadWord  ( t, n, m))) => ( is_uart_reg_addr (addres n m s) )
+   |x => F
+`; *)
+
+val mem_eq_def = Define`
+mem_eq region mem1 mem2 = 
+   (!x. x IN region ==> ((mem1 x) = (mem2 x)))
+`;
+
+val m0_r_eq_def = Define `
+m0_r_eq region s1 s2 = 
+   (mem_eq region s1.MEM s2.MEM)
+`;
+
+val m0_non_r_eq_def = Define `
+    m0_non_r_eq region s1 s2 = (
+	(s1.AIRCR = s2.AIRCR)/\
+	(s1.CCR = s2.CCR)/\
+	(s1.CONTROL = s2.CONTROL)/\
+	(s1.CurrentMode = s2.CurrentMode)/\
+	(s1.ExceptionActive = s2.ExceptionActive)/\
+	(s1.NVIC_IPR = s2.NVIC_IPR)/\
+	(s1.PRIMASK = s2.PRIMASK)/\
+	(s1.PSR = s2.PSR)/\
+	(s1.REG = s2.REG)/\
+	(s1.SHPR2 = s2.SHPR2)/\
+	(s1.SHPR3 = s2.SHPR3)/\
+	(s1.VTOR = s2.VTOR)/\
+	(s1.count = s2.count)/\
+	(s1.exception = s2.exception)/\
+	(s1.pcinc = s2.pcinc)/\
+	(s1.pending = s2.pending)/\
+	(mem_eq {x|  x NOTIN region } s1.MEM s2.MEM))`;
+
+
+
+val m0_non_uart_eq_def = Define `
+  m0_non_uart_eq s1 s2 = (m0_non_r_eq uart_region s1 s2)
+`;
+
+
+(** There is no flow to a memory region from the rest of the state 
+    During the next tranisition
+
+    for arbitrary content of the region, the next instruciton does not change the content of the region
 **)
-((ARB, ARB), ARB, ARB)`
+val no_flow_to_def = Define` 
+ no_flow_to region s = (
+  !s'. m0_non_r_eq region s s' ==> m0_r_eq region s' (Next s') 
+ )`;
 
-(********************************************)
-(*          No exceptions                   *)
-(*                                          *)
-(********************************************)
-val NEX_def = Define `
-    NEX (P :(m0_component # m0_data -> bool) -> bool) t = ! s seq i.    
-               ((SEP_REFINE (P * SEP_T) ($=) (STATE m0_proj) s) /\
-               rel_sequence (NEXT_REL $= NextStateM0) seq  s /\
-               ((seq (SUC i)).count <= s.count+ t))==>   
-	           ((seq i).count < (Next(seq i)).count) /\
-                   ((Next (seq (i))).exception = NoException) `;
-
-(********************************************)
-(*           Uart model theorems            *)
-(*                                          *)
-(********************************************)
-val AXI = Q.store_thm("AXI", `
-!s su.  
-(NIT_STEP uart_r s) /\ (m0u_m0_non_r_eq uart_r su s ) ==>
-             (m0u_m0_non_r_eq uart_r (m0u_Next su) (Next s))/\
-             (m0u_r_eq uart_r (m0u_Next su) su)`,
-
-    REPEAT GEN_TAC>> 
-    Cases_on `su`>> Cases_on `r` >> Cases_on `q`>>
-
-    SIMP_TAC (std_ss++LET_ss) [m0u_Next_def, m0u_r_eq_def ,m0u_m0_non_r_eq_def, PULL_FORALL, NIT_STEP_TRANS_thm, NIT_STEP_TRANS_thm]>>
+(** There is no information flow to the rest of the state from this region 
+    During the next tranisition 
     
-    METIS_TAC[
-NIT_STEP_TRANS_thm, m0_non_r_eq_antisym_thm,
-        m0_non_r_eq_antisym_thm,
-	m0_r_eq_antisym_thm, m0u_m0_non_r_eq_def,
-	m0u_r_eq_def, NIT_STEP_thm]
+    Swaping out the content of the region arbitraraly does not affect the execution of the rest of the state.
+**)
+val no_flow_from_def = Define` 
+ no_flow_from region s = (
+  !s'. m0_non_r_eq region s s' ==> m0_r_eq region (Next s) (Next s') 
+ )`;
+
+
+
+
+val uart_region_def = Define`
+(* TODO: change to bit masking? *)
+uart_region = {addr| addr >= 0x40002000w /\ addr <= 0x4000256Cw}
+`;
+
+
+val no_if_to_uart_def = Define`
+no_if_to_uart s = no_flow_to uart_region s`;
+
+
+val no_if_from_uart_def = Define`
+no_if_from_uart s = no_flow_from uart_region s`;
+
+
+val ward_region_def = Define`
+(* TODO: change to bit masking? *)
+ward_region x = {addr| (addr = x) \/ (addr = x+1w) \/
+                         (addr = x+2w) \/ (addr = x+3w)}
+`;
+
+val no_if_to_word_def = Define`
+no_if_to_word addr s = no_flow_to ward_region s`;
+
+
+val no_if_from_word_def = Define`
+no_if_from_word addr s = no_flow_from (ward_region addr) s`;
+=======
+val mem_region_eq_def = Define`
+mem_eq region mem1 mem2 = 
+   (!x. x IN region ==> ((mem1 x) = (mem2 x)))
+`
+
+val m0_region_eq_def = Define `
+m0_region_eq region s1 s2 = 
+   (mem_eq region s1.MEM s2.MEM)
+`
+DB.find "m0_state"
+val m0_non_region_eq_def = Define `
+  m0_non_uart_eq s1 s2 = (
+
+(s1.AIRCR = s2.AIRCR)/\
+(s1.CCR = s2.CCR)/\
+(s1.CONTROL = s2.CONTROL)/\
+(s1.CurrentMode = s2.CurrentMode)/\
+ExceptionActive
+NVIC_IPR
+PRIMASK
+PSR
+REG
+SHPR2
+SHPR3
+VTOR
+count
+exception
+pcinc
+pending
+
+   (a.REG = b.REG) /\ (a.count = b.count) /\ (non_uart_mem_eq a.MEM b.MEM)
+   (* Do we need to include other parts of the state ?, yes*)
+  )
+`;
+
+val m0_non_uart_eq_def = Define `
+  m0_non_uart_eq a b = (
+   (a.REG = b.REG) /\ (a.count = b.count) /\ (non_uart_mem_eq a.MEM b.MEM)
+   (* Do we need to include other parts of the state ?, yes*)
+  )
+`;
+
+val m0_uart_eq_def = Define `
+  m0_uart_eq a b = 
+    (uart_mem_eq a.MEM b.MEM)
+`;
+
+
+val no_if_uart_2_cpu_def = Define`
+no_if_uart_2_cpu s0 = (
+    ! s1. m0_non_uart_eq s0 s1 ==> m0_non_uart_eq (Next s0) (Next s1)
+)`;
+
+val no_if_cpu_2_uart_def = Define`
+no_if_uart_2_cpu s0 = (
+    (** we need to fex next instruction to be executed, if code is always located in a fixed region of memory then it would be better to constain that memory region instead **)
+    ! s1. (** s1.REG PC = s0.REG PC /\ s0.MEM (R s PC) = s1.MEM(R s' PC) **) => 
+         m0_uart_eq s0 s1 ==> m0_uart_eq (Next s0) (Next s1)
+)`;
+
+val no_if_2_cpu_no_load_thm = prove (`` !s.  no_if_uart_2_cpu s  ==> ~( load_uart_reg s)``,
+STRIP_TAC
+EQ_TAC
+SIMP_TAC std_ss [no_if_uart_2_cpu_def]
+Induct_on `s` 
+Induct_on `f1`
 );
 
-val _ = export_theory();
+
+(** experements to investigate proving information flow for decompiled code **)
+val m0_non_addr_eq_def = Define `
+  m0_non_uart_eq addr a b = (
+   (a.REG = b.REG) /\ (a.count = b.count) /\ 
+          (!addr'. (addr' <> addr) ==> ((a.MEM addr')=(b.MEM addr')))
+   (* Do we need to include other parts of the state ?*)
+  )
+`;
+
+
+val m0_addr_eq_def = Define `
+  m0_addr_eq addr a b =
+       (** TODO: might need to fix PC, (s.MEM PC) and regesters used by the instruction at s.MEM PC **)
+    ((a.MEM addr)=(b.MEM addr))
+`;
+
+
+(** this version without ext.quant. **)
+val mem_written_1_def = Define`
+    mem_written_1 s a = let
+      s'  = s with MEM updated_by (\m. (a =+ 0w) m );  
+      s'' = s with MEM updated_by (\m. (a =+ ~0w) m)
+    in ~((((Next(s')).MEM a) = 0w) /\ ( ((Next(s'')).MEM a)=~0w)) 
+`;
+
+(** this version is more in Information flow style**)
+
+
+val nif_from_addr_def = Define`
+    nif_from_addr a s = !s'. (** TODO: 
+                if next operation is fixed!!! ==> **) 
+         m0_addr_eq a s s' ==>
+             m0_addr_eq a (Next s) (Next s')           
+`;
+
+val nif_to_addr_def = Define`
+    nif_to_addr a s = !s'. (** TODO: 
+                if next operation is fixed!!! ==> **) 
+         m0_non_addr_eq a s s' ==>
+             m0_non_addr_eq a (Next s) (Next s')           
+`;
+
+val if_to_addr_def = Define`
+    if_to_addr_def a s = ?s'. (m0_non_addr_eq a s s' ) /\ ~(m0_non_addr_eq a (Next s) (Next s'))
+`;
