playground/uart_model_old/experements.sml
@@ -1,0 +1,143 @@
+        
+loadPath := ("/home/daniil/HOL/examples/l3-machine-code/m0/model"::(!loadPath));
+loadPath := ("/Home/daniil/HOL/examples/l3-machine-code/common"::(!loadPath));
+loadPath := ("/home/daniil/HOL/examples/l3-machine-code/m0/decompiler"::(!loadPath));
+open  wordsTheory;
+open m0Theory;
+open m0_decompLib;
+open fcpTheory;
+     
+
+EVAL ``(6w):word3``
+
+val (daniil_th, daniil_defs) = m0_decompile "daniil_test" `
+2300 (* movs r3, #0 *)`;
+
+val (daniil_th, daniil_defs) = m0_decompile "daniil_test" `
+f7ff ffe2 (* 	bl	17a <validate_seq_headers>*)`;
+
+
+DB.find "daniil_test_pre";
+
+
+
+
+uart_reg_load
+
+uart_reg_store (state, dev) = 
+DB.find "m0_REG"
+
+
+
+(* test program *)
+val q =
+   `movs r1, #0              ; accumulator
+    mov  r3, r0              ; first address
+    adds r3, #40             ; last address (10 loads)
+l1: ldr  r2, [r0, #4]        ; load data
+    adds r0, #4              ; increment address
+    add  r1, r2              ; add to accumulator
+    cmp  r0, r3              ; test if done
+    ble  l1                  ; loop if not done`
+
+
+(* test program *)
+val q =
+   `l1: bl  l1                  ; loop if not done`
+
+
+add_decompiled
+derive_individual_specs
+(* from GAS *)
+val (test_cert, test_def) = m0_decompile "test" `
+   2100
+   0003
+   3328
+   6842
+   3004
+   4411
+   4298
+   DBFA`
+
+get_decompiled "test"
+ decompiler_memory
+
+(* internal assembler *)
+val () = m0AssemblerLib.print_m0_code `
+
+m0_decompLib
+ derive_individual_specs 
+val (test2_cert, test2_def) = m0_decompile_code "test2" `
+	mov	r3, #0  `		
+	lslsne	r0, r0, #3 
+`
+val () = m0AssemblerLib.print_m0_code q
+
+m0_decompLib
+ derive_individual_specs 
+val (test2_cert, test2_def) = m0_decompile_code "test2" q
+
+val () = computeLib.add_funs [test_def]
+val () = computeLib.add_funs [test2_def]
+
+val run1 = Theory.save_thm("run1",
+  EVAL ``test (12w, 0, dmem, \a. if a && 3w = 0w then 4w else 0w)``)
+
+val run2 = Theory.save_thm("run2",
+  EVAL ``test2 (12w, 0, dmem, \a. if a && 3w = 0w then 4w else 0w)``)
+
+val () = export_theory()
+
+
+
+(** remove this **)
+open HolKernel Parse boolLib bossLib
+open decompilerLib m0_progLib m0_progTheory m0_decompTheory
+
+
+local
+   fun get_length th =
+      if sumSyntax.is_inl (m0_progLib.get_code th) then 2 else 4
+   val find_exit =
+      stateLib.get_pc_delta
+          (Lib.equal "m0_prog$m0_PC" o fst o boolSyntax.dest_strip_comb)
+   fun format_thm th = (th, get_length th, find_exit th)
+   val count_INTRO_rule =
+      stateLib.introduce_triple_definition (false, m0_COUNT_def) o
+      Thm.INST [``endianness:bool`` |-> boolSyntax.F,
+                ``spsel:bool`` |-> boolSyntax.F]
+   val finalise =
+      List.map format_thm o stateLib.fix_precond o List.map count_INTRO_rule
+in
+   val set_opt = m0_progLib.m0_config false
+   fun m0_triples hex =
+      case finalise (m0_progLib.m0_spec_hex hex) of
+         [x] => (x, NONE)
+       | [x1, x2] => (x1, SOME x2)
+       | _ => raise ERR "m0_triples" ""
+   fun m0_triples_opt s hex = (set_opt s; m0_triples hex)
+end
+
+val m0_pc = Term.prim_mk_const {Thy = "m0_prog", Name = "m0_PC"}
+
+fun m0_tools f hide = (f, fn _ => fail(), hide, m0_pc): decompiler_tools
+fun m0_tools_opt opt = m0_tools (m0_triples_opt opt)
+
+val l3_m0_tools = m0_tools m0_triples m0_NZCV_HIDE
+val l3_m0_tools_no_status = m0_tools m0_triples TRUTH
+
+val l3_m0_tools_flat = m0_tools_opt "flat" m0_NZCV_HIDE
+val l3_m0_tools_array = m0_tools_opt "array" m0_NZCV_HIDE
+val l3_m0_tools_mapped = m0_tools_opt "mapped" m0_NZCV_HIDE
+
+val l3_m0_tools_flat_no_status = m0_tools_opt "flat" TRUTH
+val l3_m0_tools_array_no_status = m0_tools_opt "array" TRUTH
+val l3_m0_tools_mapped_no_status = m0_tools_opt "mapped" TRUTH
+
+fun m0_decompile name qcode =
+   (set_opt "mapped"; decompilerLib.decompile l3_m0_tools name qcode)
+
+fun m0_decompile_code name (qass: string quotation) =
+   ( set_opt "mapped"
+   ; decompilerLib.decompile_with m0AssemblerLib.m0_code l3_m0_tools name qass
+   )
